src/Goose/base.v
@@ -1,6 +1,7 @@
 From Classes Require Import EqualDec.
 
 From RecoveryRefinement Require Export Spec.Proc.
+From RecoveryRefinement Require Export Spec.LockDefs.
 
 From RecoveryRefinement.Goose Require Export Machine.
 From RecoveryRefinement.Goose Require Export GoZeroValues.
