src/Spec/LockDefs.v
@@ -1,0 +1,45 @@
+Inductive LockStatus := Locked | ReadLocked (num:nat) | Unlocked.
+Inductive LockMode := Reader | Writer.
+
+(* returns [Some s'] when the lock should be acquired to status s', and None
+  if the lock would block *)
+Definition lock_acquire (m:LockMode) (s:LockStatus) : option LockStatus :=
+  match m, s with
+  | Reader, ReadLocked n => Some (ReadLocked (S n))
+  (* note that the number is one less than the number of readers, so that
+       ReadLocked 0 means something *)
+  | Reader, Unlocked => Some (ReadLocked 0)
+  | Writer, Unlocked => Some Locked
+  | _, _ => None
+  end.
+
+(* returns [Some s'] when the lock should be released to status s', and None if this usage is an error *)
+Definition lock_release (m:LockMode) (s:LockStatus) : option LockStatus :=
+  match m, s with
+  | Reader, ReadLocked 0 => Some Unlocked
+  | Reader, ReadLocked (S n) => Some (ReadLocked n)
+  | Writer, Locked => Some Unlocked
+  | _, _ => None
+  end.
+
+(* lock_available reports whether acquiring and releasing the lock atomically
+  would succeed; phrased as an option unit for compatibility with readSome *)
+Definition lock_available (m:LockMode) (s:LockStatus) : option unit :=
+  match m, s with
+  | Reader, ReadLocked _ => Some tt
+  | _, Unlocked => Some tt
+  | _, _ => None
+  end.
+
+
+Definition force_read_lock (s:LockStatus) : LockStatus :=
+  match s with
+  | ReadLocked n => ReadLocked (S n)
+  | _ => ReadLocked 0
+  end.
+
+Definition force_read_unlock (s:LockStatus) : LockStatus :=
+  match s with
+  | ReadLocked (S n) => ReadLocked n
+  | _ => Unlocked
+  end.
